---
title: "Summation Rules"
date: "`r Sys.Date()`"
header-includes:
   - \usepackage{amsthm}
   - \usepackage{xcolor}
   - \usepackage{xfrac}
   - \usepackage[framemethod=tikz]{mdframed}
   - \usepackage{graphicx}
   - \usepackage{rotating}
   - \usepackage{booktabs}
   - \usepackage{caption}
   - \definecolor{umn}{RGB}{153, 0, 85}
   - \definecolor{umn2}{rgb}{0.1843137, 0.4509804, 0.5372549}
   - \definecolor{myorange}{HTML}{EA6153}
output: 
  pdf_document:
    includes:
      before_body: notes.tex
    highlight: tango
    latex_engine: xelatex
    fig_width: 6
    fig_height: 6
mainfont: "Minion Pro"
sansfont: "ITC Slimbach Std Book"
monofont: "Source Code Pro"
urlcolor: "umn2"
always_allow_html: yes
bibliography: epsy8264.bib
csl: apa-single-spaced.csl
---

\frenchspacing

```{r setup, include=FALSE, message=FALSE}
knitr::opts_chunk$set(echo = FALSE)
library(dplyr)
library(knitr)
library(kableExtra)
library(sm)
```

Assume the $X$ is a random variable such that

$$
X = \{x_1, x_2, x_3, \ldots, x_n\}
$$

Then,

$$
\sum_{i=1}^n X_i = x_1 + x_2 + x_3 + \ldots + x_n
$$

To keep the notation simpler, we will just denote this as $\sum X$.

## Summation Rules

**Rule 1:** When a summation is itself a sum or difference, the summation sign may be distributed among the separate terms of the sum. That is:

$$
\sum(X + Y) = \sum X + \sum Y
$$

\begin{proof}
\[
$$
\begin{align*}
\sum(X + Y) &= (x_1 + y_1) + (x_2 + y_2) + \ldots + (x_n + y_n) \\
&= (x_1 + x_2 + \ldots x_n) + (y_1 + y_2 + \ldots y_n) \\
&= \sum X + \sum Y
\end{align*}
$$
\]
\end{proof}

**Rule 2:** The sum of a constant, $a$, is $n$ times the value of the constant.

$$
\sum(a) = na
$$

\begin{proof}
\[
$$
\begin{align*}
\sum a &= \underbrace{a + a + \ldots + a}_{n} \\
&= na
\end{align*}
$$
\]
\end{proof}

## Examples

In the following examples $X$ and $Y$ are random variables and $a$ is a constant.

1. $\sum(X + 2)$

$$
\begin{split}
\sum(X + 2) &= \sum X + \sum 2\\
&= \sum X + 2n \\
\end{split}
$$

2. $\sum(2X + 3)$

$$
\begin{split}
\sum(2X + 3) &=\sum (2X) + \sum 3 \\
&= 2\sum X + 3n \\
\end{split}
$$

3. $\sum(X - Y)^2$

$$
\begin{split}
\sum(X - Y)^2 &= \sum(X^2 - 2XY + Y^2)\\
&= \sum (X^2) - \sum(2XY) + \sum (Y^2) \\
&= \sum (X^2) - 2\sum(XY) + \sum (Y^2) \\
\end{split}
$$

